Veir/IR/Buffed/RawReadWriteLemmas/Tactics.lean
@@ -13,7 +13,7 @@ namespace Veir.Buffed
 
 section read_write
 
-variable [HasOpInfo OpInfo] [SerializableOpInfo OpInfo] {ctx : Sim.IRContext OpInfo}
+variable [HasOpInfo OpInfo] [SerializableOpInfo OpInfo] [HasBuffedProperties OpInfo] {ctx : Sim.IRContext OpInfo}
 
 /-! Tactic macros for the read/write interaction lemmas -/
 
